\begin{enumerate}[leftmargin=*]
    \item \textbf{Symmetry Rule}
        \[\binom{n}{k} = \binom{n}{n - k}\]
    
    \item \textbf{Factoring In}
        \[\binom{n}{k} = \frac{n}{k} \binom{n - 1}{k - 1}\]
    
    \item \textbf{Sum Over $k$}
        \[\sum_{k = 0}^{n} \binom{n}{k} = 2^n\]
    
    \item \textbf{Sum Over $n$}
        \[\sum_{m = 0}^{n} \binom{m}{k} = \binom{n + 1}{k + 1}\]
    
    \item \textbf{Sum Over $n$ and $k$}
        \[\sum_{k = 0}^{m} \binom{n + k}{k} = \binom{n + m + 1}{m}\]
    
    \item \textbf{Sum of the Squares}
        \[\binom{n}{0}^2 + \binom{n}{1}^2 + \cdots + \binom{n}{n}^2 = \binom{2n}{n}\]
    
    \item \textbf{Weighted Sum}
        \[1 \cdot \binom{n}{1} + 2 \cdot \binom{n}{2} + \cdots + n \cdot \binom{n}{n} = n \cdot 2^{n - 1}\]
    
    \item \textbf{Connection with Fibonacci Numbers}
        \[\binom{n}{0} + \binom{n - 1}{1} + \cdots + \binom{n - k}{k} + \cdots + \binom{0}{n} = F_{n + 1}\]
\end{enumerate}