\textbf{Binomial Coefficient Identities}
\begin{enumerate}[leftmargin=*]
    \item \textbf{Fibonacci Binomial Identity}
        \[\sum_{0\leq k \leq n} \binom{n-k}{k} = \text{Fib}_{n+1}\]
    
    \item \textbf{Symmetry Rule}
        \[\binom{n}{k} = \binom{n}{n-k}\]
    
    \item \textbf{Pascal's Recurrence}
        \[\binom{n}{k} + \binom{n}{k+1} = \binom{n+1}{k+1}\]
    
    \item \textbf{Absorption Identity}
        \[k\binom{n}{k} = n\binom{n-1}{k-1}\]
    
    \item \textbf{Factoring In}
        \[\binom{n}{k} = \frac{n}{k}\binom{n-1}{k-1}\]
    
    \item \textbf{Sum of Binomial Coefficients}
        \[\sum_{i=0}^n \binom{n}{i} = 2^n\]
    
    \item \textbf{Sum of Even Binomial Coefficients}
        \[\sum_{i\geq 0} \binom{n}{2i} = 2^{n-1}\]
    
    \item \textbf{Sum of Odd Binomial Coefficients}
        \[\sum_{i\geq 0} \binom{n}{2i+1} = 2^{n-1}\]
    
    \item \textbf{Alternating Sum Identity}
        \[\sum_{i=0}^k (-1)^i \binom{n}{i} = (-1)^k \binom{n-1}{k}\]
    
    \item \textbf{Hockey-Stick Identity}
        \[\sum_{i=0}^k \binom{n+i}{i} = \sum_{i=0}^k \binom{n+i}{n} = \binom{n+k+1}{k}\]
    
    \item \textbf{Weighted Linear Sum}
        \[\sum_{i=1}^n i\binom{n}{i} = n2^{n-1}\]
    
    \item \textbf{Weighted Quadratic Sum}
        \[\sum_{i=1}^n i^2\binom{n}{i} = (n+n^2)2^{n-2}\]
    
    \item \textbf{Vandermonde Convolution}
        \[\sum_{k=0}^r \binom{m}{k}\binom{n}{r-k} = \binom{m+n}{r}\]
    
    \item \textbf{Upward Hockey-Stick Identity}
        \[\sum_{i=r}^n \binom{i}{r} = \binom{n+1}{r+1}\]
    
    \item \textbf{Sum of Squared Binomial Coefficients}
        \[\sum_{i=0}^k \binom{k}{i}^2 = \binom{2k}{k}\]
    
    \item \textbf{Chu-Vandermonde Special Case}
        \[\sum_{i=1}^n \binom{n}{i}\binom{n-1}{i-1} = \binom{2n-1}{n-1}\]
    
    \item \textbf{Double Subset Selection}
        \[\sum_{k=q}^n \binom{n}{k}\binom{k}{q} = 2^{n-q}\binom{n}{q}\]
    
    \item \textbf{Generalized Binomial Theorem}
        \[\sum_{i=0}^n k^i\binom{n}{i} = (k+1)^n\]
    
    \item \textbf{Half Binomial Sum}
        \[\sum_{i=0}^n \binom{2n}{i} = 2^{2n-1} + \frac{1}{2}\binom{2n}{n}\]
    
    \item \textbf{Squared Central Binomial Sum}
        \[\sum_{i=0}^n \binom{2n}{i}^2 = \frac{1}{2}\left(\binom{4n}{2n} + \binom{2n}{n}^2\right)\]
\end{enumerate}