\begin{enumerate}[leftmargin=*]
    \item \textbf{Definition}
        \begin{itemize}
            \item $F_0 = 0,\ F_1 = 1$
            \item $F_n = F_{n-1} + F_{n-2}$ for $n \geq 2$
        \end{itemize}
    
    \item \textbf{Combinatorial Formula}
        \[F_n = \sum_{k=0}^{\lfloor\frac{n-1}{2}\rfloor} \binom{n-k-1}{k}\]
    
    \item \textbf{Binet's Formula}
        \[F_n = \frac{1}{\sqrt{5}}\left(\frac{1+\sqrt{5}}{2}\right)^n - \frac{1}{\sqrt{5}}\left(\frac{1-\sqrt{5}}{2}\right)^n\]
    
    \item \textbf{Sum of First $n$ Fibonacci Numbers}
        \[\sum_{i=1}^n F_i = F_{n+2} - 1\]
    
    \item \textbf{Sum of Odd-indexed Fibonacci Numbers}
        \[\sum_{i=0}^{n-1} F_{2i+1} = F_{2n}\]
    
    \item \textbf{Sum of Even-indexed Fibonacci Numbers}
        \[\sum_{i=1}^n F_{2i} = F_{2n+1} - 1\]
    
    \item \textbf{Sum of Squares}
        \[\sum_{i=1}^n F_i^2 = F_n F_{n+1}\]
    
    \item \textbf{Cassini's Identity}
        \[F_m F_{n+1} - F_{m-1} F_n = (-1)^n F_{m-n}\]
        \[F_{2n} = F_{n+1}^2 - F_{n-1}^2 = F_n(F_{n+1} + F_{n-1})\]
    
    \item \textbf{Addition Formulas}
        \[F_m F_n + F_{m-1} F_{n-1} = F_{m+n-1}\]
        \[F_m F_{n+1} + F_{m-1} F_n = F_{m+n}\]
    
    \item \textbf{Fibonacci Test}
        \begin{itemize}
            \item A natural number $n$ is Fibonacci iff $5n^2 + 4$ or $5n^2 - 4$ is a perfect square
        \end{itemize}
    
    \item \textbf{Divisibility Property}
        \begin{itemize}
            \item Every $k$-th Fibonacci number is a multiple of $F_k$
        \end{itemize}
    
    \item \textbf{GCD Property}
        \[\gcd(F_m, F_n) = F_{\gcd(m,n)}\]
    
    \item \textbf{Coprimality}
        \begin{itemize}
            \item Any three consecutive Fibonacci numbers are pairwise coprime
        \end{itemize}
    
    \item \textbf{Periodicity Modulo $n$}
        \begin{itemize}
            \item Fibonacci sequence modulo $n$ is periodic with Pisano period $\leq 6n$
        \end{itemize}
\end{enumerate}